Logic.v
@@ -37,8 +37,67 @@ gives us emp, *, -*, etc.  ClassicalSep tell us P * emp = P etc..  **)
   Parameter SRm: SepRec mpred.  Existing Instance SRm.
   Parameter mapsto: forall (a: loc)(v: value), mpred.
                          
+  (* Definition assert := w -> mpred. *)
+  Inductive assert : world -> Prop := 
+  | tt_a  : assert
+  | eq_a  : expr -> expr -> assert
+  | not_a : assert -> assert
+  | and_a : assert -> assert -> assert.
   
-  Definition assert := world -> mpred.
+  Fixpoint eval_assert a :=
+    match a with
+      | tt_a => fun w => True
+      | eq_a e1 e2 => fun w => eval w e1 = eval w e2
+      | not_a p => fun w => (eval_assert p w -> False)
+      | and_a p q => fun w => eval_assert p w /\ eval_assert q w
+      (* | or_a p q => eval_assert w p \/ eval_assert w q *)
+      (* | imp_a p q => eval_assert w p -> eval_assert w q *)
+      (* | ex_a p   => exists e, eval_assert w (p e) *)
+      (* | all_a p   => forall e, eval_assert w (p e) *)
+    end.
+  
+  Definition pred : assert -> (world -> Prop) := fun a => eval_assert a.
+  
+  Definition derives_pred (p q : pred) : Prop :=
+    forall w , pred p w -> pred q w.
+  
+  Lemma derives_trans : 
+    forall p q r, derives_pred p q -> derives_pred q r -> derives_pred p r.
+  Proof.
+    firstorder.
+  Qed.
+
+  Lemma derives_refl : 
+    forall p, derives_pred p p.
+  Proof.
+    firstorder.
+  Qed.
+  
+  Lemma pred_ext : forall p q,
+                       derives_pred p q -> derives_pred q p -> p = q.
+  Proof.
+    intros.
+    extensionality.
+    apply prop_ext.
+    firstorder.
+  Qed.
+
+
+  Parameter assert_ext: forall a b, derives_assert a b -> derives_assert b a -> a = b.
+  Axiom assert_refl : forall a, derives_assert a a.
+  
+  Instance Foo : NatDed assert.  
+  Proof.
+    eapply (mkNatDed assert and_a or_a 
+                     ex_a all_a
+                     imp_a
+                     prop_a
+                     derives_assert
+                     assert_ext
+                     assert_refl
+           ).
+    intros.
+    
 
   Definition pure{A : Type} {N : NatDed A } {S : SepLog A} (P : A) := P |-- emp.
   Axiom sepcon_pure_andp : forall {A : Type} {N : NatDed A} {S : SepLog A} (P Q : A), pure P -> pure Q -> ((P * Q) = (P && Q)).
@@ -76,7 +135,7 @@ gives us emp, *, -*, etc.  ClassicalSep tell us P * emp = P etc..  **)
   (* Definition nonfreevars (P: assert) (x: var) : Prop := *)
   (*     P |-- (ALL v : _, subst_pred (subst_one x v) P). *)
   Definition nonfreevars (P: assert) (x: var) : Prop :=
-    forall v, (P |-- subst_pred (subst_one x v) P).
+    forall v, (P = subst_pred (subst_one x v) P).
   
   Definition procspec := (pname * proc * assert * assert)%type.
   Definition procspecs := list procspec.
