TranslationLemmas.v
@@ -11,1302 +11,970 @@ Require Import Subst.
 Require Import ProgramLogic.
 Require Import Translation.
 Require Import Language.
-Require Import WFLemmas.
-Require Import SubstLemmas.
-Require Import EvalLemmas.
-Require Import Tactics.
-Require Import List.
+
+(* Require Import WFLemmas. *)
+(* Require Import SubstLemmas. *)
+(* Require Import EvalLemmas. *)
+(* Require Import Tactics. *)
+(* Require Import List. *)
 Import ListNotations.
 
-Lemma forall_p_combine :
-  forall (X Y : Type) (P : Y -> Prop) (xs : list X) (ys : list Y),
-    length xs = length ys ->
-    Forall P ys -> 
-    Forall (fun xy => P (snd xy)) (combine xs ys).
+(* Lemma forall_p_combine : *)
+(*   forall (X Y : Type) (P : Y -> Prop) (xs : list X) (ys : list Y), *)
+(*     length xs = length ys -> *)
+(*     Forall P ys ->  *)
+(*     Forall (fun xy => P (snd xy)) (combine xs ys). *)
+(* Proof. *)
+(*   intros. *)
+(*   rewrite Forall_forall in *. *)
+(*   intros. *)
+(*   destruct x as [x y]. *)
+(*   simpl in *. *)
+(*   pose (combine_split xs ys H). *)
+(*   specialize (H0 y). *)
+(*   apply in_combine_r in H1. *)
+(*   apply H0. *)
+(*   assumption. *)
+(* Qed. *)
+
+Lemma subst_emp_id :
+  forall s,
+    subst_pred s emp = emp.
 Proof.
-  intros.
-  rewrite Forall_forall in *.
-  intros.
-  destruct x as [x y].
-  simpl in *.
-  pose (combine_split xs ys H).
-  specialize (H0 y).
-  apply in_combine_r in H1.
-  apply H0.
-  assumption.
+  normalize.
 Qed.
 
-Lemma sub_eq_expr :
-  forall (e : expr) x x', 
-    subst (subst_one x (var_e x')) e 
-    = subst (fun i => if eq_dec i x then x' else i) e.
+Hint Resolve subst_emp_id : subst.
+
+Lemma vv_not_fv :
+  forall G Gr H e T,
+    wf_env H G -> expr_type G H Gr e T -> ~ FV e ν.
+Proof.
+  intros.
+  induction H1; eauto with datatypes.
+  + induction Γ.
+    contradiction H.
+    apply in_inv in H.
+    destruct a as [x' [b' p']].
+    destruct H. inversion H. subst.
+    inversion H0. subst.
+    unfold FV.
+    unfold fv_expr.
+    intro.
+    inversion H1. subst x. apply H5. reflexivity. contradiction.
+    apply IHΓ. inversion H0. assumption. assumption.
+Qed.
+
+Lemma fresh_var_cons :
+  forall G H xt x, fresh x (xt :: G) H -> fresh x G H.
+Proof. 
+  firstorder. 
+  unfold var_not_in in *.
+  rewrite Forall_forall in *.
+  intros.
+  apply H1.
+  eauto with datatypes.
+Qed.
+  
+Lemma fresh_var_nonmem_env :
+  forall G H x, fresh x G H -> var_not_in x G.
+Proof.
+  firstorder.
+Qed.
+
+Lemma fresh_var_nonmem_heap :
+  forall G H x, fresh x G H -> bind_not_in x H.
+Proof.
+  firstorder.
+Qed.
+
+Lemma var_not_in_not_eq :
+  forall G x x' t, var_not_in x ((x',t) :: G) -> x' <> x.
+Proof.
+  intros.
+  unfold var_not_in in *.
+  rewrite Forall_forall in *.
+  specialize (H (x',t)).
+  apply H.
+  left.
+  reflexivity.
+Qed.
+
+Lemma bind_not_in_not_eq :
+  forall H v l x t, bind_not_in v ((l,(x,t)) :: H) -> x <> v.
+Proof.
+  intros.
+  unfold bind_not_in in *.
+  rewrite Forall_forall in *.
+  specialize (H0 (l,(x,t))).
+  apply H0.
+  eauto with datatypes.
+Qed.
+
+Lemma var_not_in_and_in :
+  forall G x, var_not_in x G -> ~ (var_in x G).
+Proof.
+  unfold var_not_in.
+  unfold var_in.
+  intros.
+  rewrite Forall_forall in *.
+  firstorder.
+Qed.
+
+Lemma bind_not_in_and_in :
+  forall H x, bind_not_in x H <-> ~ (bind_in x H).
+Proof.
+  intros.
+  unfold bind_not_in, bind_in.
+  rewrite Forall_forall.
+  firstorder.
+  intro.
+  subst x.
+  destruct x0 as [l [x t]].
+  apply (H0 l).
+  exists t.
+  apply H1.
+Qed.
+
+Hint Resolve 
+     fresh_var_nonmem_env
+     fresh_var_nonmem_heap
+     var_not_in_not_eq 
+     var_not_in_and_in
+     bind_not_in_and_in
+     fresh_var_cons
+     vv_not_fv
+: var.
+
+Lemma subst_dist_sepcon :
+  forall P Q (s : var -> expr),
+    subst_pred s (P * Q) = subst_pred s P * subst_pred s Q.
+Proof.
+  firstorder.
+Qed.
+
+Lemma subst_dist_andp :
+  forall P Q (s : var -> expr),
+    subst_pred s (P && Q) = subst_pred s P && subst_pred s Q.
+Proof.
+  firstorder.
+Qed.
+
+Lemma subst_dist_orp :
+  forall P Q (s : var -> expr),
+    subst_pred s (P || Q) = subst_pred s P || subst_pred s Q.
+Proof.
+  firstorder.
+Qed.
+
+Lemma subst_dist_imp :
+  forall P Q (s : var -> expr),
+    subst_pred s (P --> Q) = subst_pred s P --> subst_pred s Q.
+Proof.
+  firstorder.
+Qed.
+
+Lemma fresh_var_expr_fv :
+  forall G H e x, 
+    fresh x G H -> wf_expr G H e -> FV e x -> False.
 Proof.
   induction e.
-  * reflexivity.
-  * intros. unfold subst. simpl. unfold subst_one. foo. 
-  * intros.
-    unfold subst at 1.
-    unfold Subst_var_expr.
-    unfold Language.subst_expr.
+  + firstorder.
+  + firstorder.
+    inversion H1; subst.
+    inversion H1; subst. 
+      eapply var_not_in_and_in; eauto.
+      eapply bind_not_in_and_in; eauto.
+      congruence.
+      eapply bind_not_in_and_in; eauto.
+      congruence.
+  + intro x.
+    unfold FV in *.
+    intros.
+    simpl in *.
+    apply in_app_or in H2.
+    inversion H1; subst.
+    destruct H2.
+    eapply IHe1; eauto.
+    eapply IHe2; eauto.
+Qed.
+
+Lemma nonfree_var_expr_eval :
+  forall e e' x,
+    (FV e x -> False) ->
+    forall w,
+      (eval (fun i : var => eval w (subst_one x e' i), hp w) e = eval w e).
+Proof.
+  unfold FV.
+  intros.
+  induction e.
+  + firstorder.
+  + simpl. unfold subst_one.
+    destruct (eq_dec v x); simpl.
+    subst v.
+    contradiction H. left. reflexivity.
+    reflexivity.
+  + simpl.
     rewrite IHe1.
     rewrite IHe2.
     reflexivity.
+    intro. apply H. simpl. apply in_or_app. right. assumption.
+    intro. apply H. simpl. apply in_or_app. left. assumption.
 Qed.
-  
-Lemma sub_eq :
-  forall (p : reft_prop) x x', 
-    subst (subst_one x (var_e x')) p 
-    = subst (fun i => if eq_dec i x then x' else i) p.
+
+Lemma fresh_var_nonfree_pred :
+  forall G H p x,
+    fresh x G H -> wf_prop G H p -> nonfreevars (sep_pred p) x.
 Proof.
   intros.
   induction p.
-  constructor.
-  unfold subst.
-  unfold Subst_prop, Subst_prop_var, subst_prop, subst_prop_var.
-  rewrite sub_eq_expr.
-  rewrite sub_eq_expr.
-  reflexivity.
-  unfold subst in *.
-  simpl.
-  rewrite IHp.
-  reflexivity.
-  unfold subst in *.
-  simpl.
-  rewrite IHp1.
-  rewrite IHp2.
-  reflexivity.
-  unfold subst in *.
-  simpl.
-  rewrite IHp1.
-  rewrite IHp2.
-  reflexivity.
-Qed.
-
-Lemma subst_vv_ty:
-  forall x x' T,
-    x <> ν ->
-    sep_ty (var_e x) T 
-    |-- subst (subst_one ν x') (sep_ty (var_e x) T).
-Proof.
-  intros.
-  unfold subst.
-  unfold sep_ty.
-  destruct T as [b p].
-  rewrite subst_distr_andp.
-  apply andp_derives.
-  rewrite subst_distr_andp.
-  apply andp_derives.
-  unfold sep_base.
-  unfold subst, Subst_pred, subst_pred.
-  simpl in *.
-  intro w.
-  apply exp_left.
-  intro vv.
-  rewrite <- exp_andp1.
-  apply andp_derives.
-  normalize.
-  apply (exp_right vv).
-  apply prop_right.
-  unfold subst_one. 
-  destruct (eq_dec x ν).
-    congruence.
-    rewrite <- H0. reflexivity.
-  apply derives_refl.
-  intro w.
-  unfold subst at 2, Subst_pred, subst_pred.
-  repeat rewrite <- subst_ty_prop.
-  unfold subst, Subst_pred, subst_pred.
-  assert
-     ((λ i : var, eval w (subst_one ν (var_e x) i))
-      = (λ i : var,
-               eval (fun i0 => eval w (subst_one ν x' i0), hp w)
-                    (subst_one ν (var_e x) i))).
-  extensionality i.
-  unfold subst_one. 
-  destruct (eq_dec i ν). 
-  simpl.
-  destruct (eq_dec x ν). intuition. reflexivity.
-  destruct (eq_dec i ν). intuition. simpl.
-  destruct (eq_dec i ν). intuition. reflexivity.
-  rewrite <- H0.
-  simpl.
-  apply derives_refl.
-  normalize.
-Qed.
- 
-Lemma vv_sub_env :
-  forall G,  
-    var_not_in ν G -> 
-      (forall x,
-         sep_env G |-- subst (subst_one ν x) (sep_env G)).
-Proof.
-  intro G.
-  induction G.
-  + simpl. trivial.
-  + destruct a as [b p].
-    unfold sep_env in *.
-    fold sep_env in *.
-    intro H.
-    intro e.
-    repeat rewrite subst_distr_andp.
-    apply andp_derives.
-    apply andp_derives.
-    apply subst_vv_ty.
-    unfold var_not_in in H.
-    rewrite Forall_forall in H.
-    apply H with (x := (b, p)).
-    left. reflexivity.
-    apply IHG.
-    inversion H.
-    assumption.
-    trivial.
-Qed.
-
-Lemma vv_sub_guards :
-  forall G Grds,
-    wf_guards G Grds -> 
-      forall (x : expr),
-      sep_guards Grds |-- subst (subst_one ν x) (sep_guards Grds).
-Proof.
-  intros G Grds.
-  induction Grds as [| p].
-  + simpl. trivial.
-  + intros wf x.
-    unfold sep_guards in *; fold sep_guards in *.
-    inversion wf. subst.
-    pose (wf_guards_vv_nonfree G Grds H2).
-    repeat rewrite subst_distr_andp.
-    repeat apply andp_derives.
-    rewrite subst_nonfree_prop.
-    apply derives_refl.
-    apply H1.
-    apply n.
-    trivial.
-Qed.
-
-Lemma subtype_interp_pred :
-  forall Γ Ξ φ φ' x b,
-    var_not_in ν Γ ->
-    wf_guards Γ Ξ -> 
-    subtype Γ Ξ { ν : b | φ } { ν : b | φ' } -> 
-    (sep_env Γ && sep_guards Ξ) |-- 
-      sep_pred (subst (subst_one ν x) φ) --> 
-      sep_pred (subst (subst_one ν x) φ').
-Proof.
-  intros.
-  inversion H1. subst.
-  simpl.
-  intro.
-  rewrite <- (subst_ty_prop φ (subst_one ν x) x0).
-  rewrite <- (subst_ty_prop φ' (subst_one ν x) x0).
-  apply derives_trans with
-    (Q := subst (subst_one ν x) (sep_env Γ) x0 &&
-          subst (subst_one ν x) (sep_guards Ξ) x0).
-  apply andp_derives.
-  apply vv_sub_env; assumption.
-  apply vv_sub_guards with (G := Γ); assumption.
-  unfold subst, Subst_pred, subst_pred.
-  simpl in H5.
-  apply H5.
-Qed.
-
-Lemma subtype_interp :
-  forall Γ Ξ φ φ' x b,
-    var_not_in ν Γ ->
-    wf_guards Γ Ξ ->
-    subtype Γ Ξ { ν : b | φ } { ν : b | φ' } -> 
-      sep_env Γ && sep_guards Ξ |-- 
-              sep_ty x { ν : b | φ } --> sep_ty x { ν : b | φ' }.
-Proof.
-  intros.
-  unfold sep_ty.
-  rewrite <- imp_andp_adjoint.
-  repeat apply andp_right.
-  apply andp_left2. apply andp_left1. apply andp_left1. apply derives_refl.
-  apply derives_trans with (Q := (sep_pred (subst (subst_one ν x) φ) 
-                              && (sep_pred (subst (subst_one ν x) φ) 
-                                 --> sep_pred (subst (subst_one ν x) φ')))).
-  apply andp_right.
-  apply andp_left2. apply andp_left1. apply andp_left2. apply derives_refl.
-  apply andp_left1. apply subtype_interp_pred with (b := b); assumption.
-  apply modus_ponens.
-  repeat apply andp_left1.
-  apply sep_env_pure.
-Qed.
-
-Lemma heap_subtype_interp :
-  forall Γ Ξ Σ Σ',
-    wf_guards Γ Ξ ->
-    heap_subtype Γ Ξ Σ Σ' ->
-    sep_env Γ && sep_guards Ξ |-- sep_heap Σ --> sep_heap Σ'.
-Proof.
-  intros.
-  rewrite <- imp_andp_adjoint.
-  unfold heap_subtype in *.
-  unfold sep_heap.
-  induction Σ.
-  destruct Σ'.
-  apply andp_left2. apply derives_refl.
-  destruct H0.
-  unfold eq_dom in H0.
-  destruct (H0 (fst p)).
-  exfalso. unfold loc_in in H3. exists (snd p). left. destruct p. reflexivity.
-  inversion H3.
-  destruct Σ'.
-  destruct H0.
-  unfold eq_dom in H0.
-  destruct (H0 (fst a)).
-  unfold loc_in in H2. 
-  destruct H2. exists (snd a). left. destruct a. reflexivity. inversion H2.
-  unfold sep_heap. fold sep_heap.
-
-Lemma vv_sub_env_eval :
-  forall e ν x v w,
-    x <> ν -> 
-    eval w (subst (subst_one ν (var_e x)) e)
-    = eval (λ i : var, eval w (subst_one ν v i), hp w) (subst (subst_one ν (var_e x)) e).
-Proof.
-  induction e.
-  + intros. unfold subst, subst_one. reflexivity.
-  + intros. unfold subst, subst_one.
-    foo.
-  + intros. unfold subst, subst_one in *. 
-            unfold Subst_var_expr, subst_var, Language.subst_expr.
-            simpl in *.
-            unfold Subst_var_expr in *.
-            rewrite IHe1 with (v:=v).
-            rewrite IHe2 with (v:=v).
-            reflexivity.
-            assumption.
-            assumption.
-Qed.
-
-Lemma vv_sub_env_prop :
-  forall p ν x v w,
-    x <> ν ->
-    sep_pred (subst (subst_one ν (var_e x)) p) w =
-    sep_pred (subst (subst_one ν (var_e x)) p)
-             (λ i : var, eval w (subst_one ν v i), hp w).
-Proof.
-  intros.
-  induction p.
-  + constructor.
-  + destruct b. unfold subst, Subst_prop, subst_prop. simpl.
-    rewrite <- vv_sub_env_eval with (v := v).
-    rewrite <- vv_sub_env_eval with (v := v).
-    reflexivity.
-    assumption.
-    assumption.
-  + simpl in *. unfold subst in *. unfold imp.
-    rewrite IHp.
-    reflexivity.
-  + simpl. unfold subst, Subst_prop in *. 
-    unfold andp.
-    rewrite IHp1.
-    rewrite IHp2.
-    reflexivity.
-  + simpl. unfold subst, Subst_prop in *. 
-    unfold orp.
-    rewrite IHp1.
-    rewrite IHp2.
-    reflexivity.
-Qed.
-
-Lemma vv_sub_env_ty :
-  forall T x v,
-    x <> ν ->
-    sep_ty (var_e x) T |-- subst (subst_one ν v) (sep_ty (var_e x) T).
-Proof.
-  intros.
-  unfold sep_ty in *.
-  destruct T as [b p].
-  repeat rewrite subst_distr_andp.
-  repeat apply andp_derives.
-  unfold subst. 
-  unfold Subst_pred, subst_pred, subst_one.
-  unfold sep_base.
-  apply exp_left.
-  intro vv.
-  simpl.
-  intro w.
-  rewrite <- exp_andp1.
-  apply andp_derives.
-  apply prop_left.
-  intro EQ.
-  apply (exp_right vv).
-  apply prop_right.
-  destruct (eq_dec x ν). intuition. assumption.
-  trivial.
-  intro w.
-  rewrite vv_sub_env_prop with (v:= v).
-  apply derives_refl.
-  assumption.
-  trivial.
-Qed.
-
-Lemma subst_vv_env :
-  forall Γ,
-    var_not_in ν Γ ->
-    nonfreevars (sep_env Γ) ν.
-Proof.
-  intros.
-  induction Γ.
-  + unfold nonfreevars. intro. apply derives_refl.
-  + unfold sep_env. destruct a as [x [b p]].
-    fold sep_env.
+  + firstorder.
+  + inversion H1; subst.
     unfold nonfreevars.
-    intro e.
-    repeat rewrite subst_distr_andp.
-    repeat apply andp_derives.
-    apply vv_sub_env_ty.
-      unfold var_not_in in H.
-      rewrite Forall_forall in H.
-      apply (H (x, { ν : b | p })); left; reflexivity.
-    apply IHΓ.
-    inversion H.
-    assumption.
-    trivial.
-Qed.
-
-Lemma sep_env_base_var :
-  forall Γ x b p,
-    (x, { ν : b | p }) ∈ Γ ->
-    sep_env Γ |-- sep_base (var_e x) b.
-Proof.
-  induction Γ.
-  + intros. inversion H.
-  + intros. 
-    apply in_inv in H. 
-    destruct a as [x' [b' p']].
-    destruct H.
-    inversion H. subst.
-    apply andp_left1.
-    apply andp_left1.
-    apply andp_left1.
-    apply andp_left1.
-    apply derives_refl.
-    unfold sep_env; fold sep_env.
-    apply andp_left1.
-    apply andp_left2.
-    apply (IHΓ _ _ p).
-    assumption.
-Qed.
-
-Lemma sep_env_base_val :
-  forall Γ (v : value),
-    sep_env Γ |-- sep_base v (base_of_val v).
-Proof.
-  intros.
-  unfold sep_base.
-  destruct (base_of_val v), v.
-  unfold base_of_type.
-  apply (exp_right n).
-  simpl. intro. apply andp_right. apply prop_right. reflexivity.
-  apply sep_env_pure.
-Qed.
-
-Lemma type_interp :
-  forall Γ Ξ x T,
-    var_not_in ν Γ ->
-    expr_type Γ Ξ x T ->
-    wf_guards Γ Ξ -> 
-    sep_env Γ && sep_guards Ξ |-- sep_ty x T.
-Proof.
-  intros Γ Ξ x T vvnotin ET. (* [ ν b φ ]  w SE ET. *)
-  unfold sep_ty.
-  dependent induction ET.
-  {
-    intros wfg.
-    apply andp_right.
-    apply andp_right.
-    apply andp_left1. 
-    apply sep_env_base_val.
-    intro w.
-    simpl.
-    apply andp_right.
-    apply prop_right.
-    unfold subst, Subst_var_expr, subst_one. simpl. foo.
-    apply andp_left1; apply sep_env_pure.
-    apply andp_left1; apply sep_env_pure.
-  }
-  {
-    intros wfg.
-    apply andp_right.
-    apply andp_right.
-  * apply andp_left1; apply sep_env_base_var with (p := φ); assumption.
-  * clear wfg.
-    apply andp_left1.
-    induction Γ.
-    + intuition.
-    + intros. 
-      destruct a as [x' [ b' p' ]].
-      apply in_inv in H.
-      destruct H.
-      inversion H; subst.
-      unfold sep_env; fold sep_env.
-      apply andp_left1.
-      apply andp_left1.
-      apply andp_left1.
-      apply andp_left2.
-      solve [intuition].
-      unfold sep_env; fold sep_env.
-      apply andp_left1.
-      apply andp_left2.
-      apply IHΓ.
-      inversion vvnotin. assumption.
-      assumption.
-   * apply andp_left1; apply sep_env_pure.
-  }
-  {
-    fold (sep_ty e T) in IHET.
-    fold (sep_ty e T').
-    intro.
-    apply derives_trans with (Q := sep_env Γ && sep_guards Ξ && sep_ty e T).
-    apply andp_right.
-    apply andp_right.
-      apply andp_left1; apply derives_refl.
-      apply andp_left2; apply derives_refl.
-      apply IHET; assumption.
-    apply imp_andp_adjoint.
-    destruct T, T'. inversion H0. subst.
-    apply subtype_interp; assumption.
-  }
-Qed.
-
-Lemma types_interp :
-  forall Γ Ξ xs ts,
-    var_not_in ν Γ ->  
-    wf_guards Γ Ξ ->
-    tc_list Γ Ξ (combine xs ts) ->
-    sep_env Γ && sep_guards Ξ |-- sep_env (combine xs ts).
-Proof.
-  intros.
-  unfold tc_list in H1.
-  rewrite Forall_forall in H1.
-  unfold sep_env.
-  induction (combine xs ts).
-  + normalize. apply andp_left1. apply sep_env_pure.
-  + destruct a. 
-    fold sep_env.
-    apply andp_right.
-    apply andp_right.
-    apply type_interp with (Γ := Γ);
-      [ assumption | apply H1 with (x := (v,r)); left; reflexivity | assumption].
-    apply IHl. 
-    intro. intro.
-    apply H1.
-    unfold In. right. apply H2.
-    apply andp_left1; apply sep_env_pure.
-Qed.
-
-Lemma funspec_nomem :
-  forall Φ p, 
-    fun_not_in p Φ ->
-    Forall (fun ps => fst4 ps <> p) (sep_proc_env Φ).
-Proof.
-  intros.
-  induction Φ.
-  + constructor.
-  + rewrite Forall_forall in *.
-    intros [ [[p' pr] P] Q ] mem.
-    destruct a as [p'' [s t]].
-    unfold sep_proc_env in mem. fold sep_proc_env in mem.
-    apply in_inv in mem.
-    destruct mem.
-    simpl in *.
-    unfold sep_schema in H0.
-    destruct t.
-    destruct s_ret.
-    inversion H0. subst.
-    unfold fun_not_in in H.
-    rewrite Forall_forall in H.
-    specialize (H (p', (s, {| s_formals := s_formals; s_formal_ts := s_formal_ts; s_ret := (v,r) |}))).
-    apply H.
-    left. reflexivity.
-    apply IHΦ.
-    inversion H. assumption.
-    assumption.
-Qed.
-    
-Lemma funspec_interp :
-  forall F f p t,
-    In (f, (p,t)) F -> In (sep_schema f p t) (sep_proc_env F).
-Proof.
-  intros.
-  induction F.
-  + inversion H.
-  + destruct H. destruct a. destruct p1. inversion H. subst.
-    apply in_inv. left. reflexivity.
-    apply IHF in H.
-    unfold sep_proc_env.
-    destruct a.
-    destruct p1.
-    simpl.
-    right.
-    apply H.
-Qed.
-(* Lemma sep_pred_pure : *)
-(*   forall p Q, *)
-(*     (sep_pred p && emp) && Q = sep_pred p * Q. *)
-(* Proof. *)
-(*   intros. *)
-(*   induction p. *)
-(*   simpl. *)
-(*   extensionality. *)
-(*   rewrite <- sepcon_emp at 1. *)
-(*   rewrite sepcon_comm. *)
-(*   apply pred_ext. *)
-(*   apply sepcon_derives. *)
-(*   apply prop_right. trivial. *)
-(*   apply andp_left2. apply derives_refl. *)
-  
-(*   unfold pure. *)
-(*   induction p. *)
-(*   simpl.  *)
-(*   repeat intro. *)
-(*   repeat (unfold join, Join_fun, Join_lower, Join_discrete in H0; hnf in H0). *)
-(*   destruct H0. *)
-(*   destruct a. destruct a0. destruct b. *)
-(*   unfold TT, prop in H. simpl in H. *)
-(*   unfold pure. *)
-
-(*   unfold identity. *)
-(*   hnf. *)
-(*   repeat intro. *)
-
-(*   unfold join in H0. *)
-(*   unfold Join_world in H0. *)
-(*   destruct a. *)
-(*   destruct a0. *)
-(*   destruct b.  *)
-(*   simpl in H0. *)
-(*   hnf in H0. *)
-(*   destruct H0. *)
-(*   simpl in *. *)
-(*   unfold join in *. *)
-(*   hnf in *. *)
-(*   unfold join, Join_equiv in *. *)
-(*   unfold join, Join_lower, Join_discrete in H1. *)
-(*   destruct H0 with (x := V 0). *)
-  
-
-Lemma sep_ty_pure_subst :
-  forall x t θ,
-    pure (subst θ (sep_ty x t)).
-Proof.
-  intros.
-  unfold pure.
-  destruct t.
-  unfold subst, sep_ty, Subst_pred, subst_pred.
-  intro w.
-  simpl.
-  apply andp_left2.
-  trivial.
-Qed.
-
-(* Lemma sep_env_pure : *)
-(*   forall G, *)
-(*     pure (sep_env G). *)
-(* Proof. *)
-(*   intros. *)
-(*   unfold pure. *)
-(*   intro. intro. *)
-(*   unfold identity. *)
-(*   intros w1 w2. *)
-(*   intros. *)
-(*   apply H0. *)
-(* Qed. *)
-
-(* Lemma sep_guards_pure : *)
-(*   forall G, *)
-(*     pure (sep_guards G). *)
-(* Proof. *)
-(*   unfold pure. *)
-(*   unfold identity. *)
-(*   intros. *)
-(*   intro. *)
-(*   intro. *)
-(*   intros w1 w2. *)
-(*   intro. *)
-(*   apply H0. *)
-(* Qed. *)
-
-Lemma sep_proof_skip :
-  forall Φ Ξ Γ Γ' (J : (Φ ; Γ ; Ξ) ⊢ skip_s ::: Γ'), 
-    sep_proc_env Φ |- {{ sep_env Γ * sep_guards Ξ }} skip_s {{ sep_env Γ' * sep_guards Ξ }}.
-Proof.
-  intros. inversion J. subst. constructor.
-Qed.
-
-Lemma sep_proof_assign :
-  forall Φ Ξ Γ Γ' x e (J : (Φ ; Γ ; Ξ)⊢ assign_s x e ::: Γ'), 
-    wf_env Γ ->
-    wf_guards Γ Ξ ->
-    sep_proc_env Φ |- {{ sep_env Γ * sep_guards Ξ }} assign_s x e {{ sep_env Γ' * sep_guards Ξ }}.
-Proof.
-  intros Φ Ξ Γ Γ' x e J wfenv wfguards.
-  inversion J. subst.
-  apply semax_frame.
-  apply semax_pre_post with (P' := (EX v : value, (eval_to e v))
-                                              && (subst_pred (subst_one x e )
-                                                             (sep_env ((x, {ν : τ | (var_e ν) .= e }) :: Γ))))
-                            (Q' := sep_env ((x,{ν : τ | (var_e ν) .= e }) :: Γ)).
-  apply andp_right.
-  unfold eval_to.
-  simpl.
-  intro w.
-  rewrite <- exp_andp1.
-  apply andp_right.
-  apply (expr_eval Γ Ξ e τ φ H7).
-  purity.
-  apply derives_trans with (Q := sep_env Γ && subst_pred (subst_one x e) (sep_env Γ)).
-  simpl. intro w.
-  rewrite subst_dom_env. 
-    apply andp_right; trivial.
-    assumption.
-    split. unfold subst_one. foo.
-    intros x' x'_in.
-    unfold subst_one. destruct (eq_dec x' x). subst.
-    unfold var_in, var_not_in in *.
-    rewrite Forall_forall in *.
-    destruct x'_in.
-    apply H5 in H.
-    contradiction H. reflexivity. reflexivity.
-    unfold subst_one. destruct (eq_dec ν x); congruence.
-  apply subst_env_eq_expr with (Grds := Ξ) (φ := φ).
-  assumption.
-  apply derives_refl.
-  rewrite exp_andp1.
-  apply semax_assign with (e := e) (x := x) (P := (sep_env ((x, {ν : τ | var_e ν .= e}) :: Γ))).
-  unfold subset.
-  intros.
-  inversion H. subst.
-  apply wf_guards_nonfree with (Γ := Γ); assumption.
-Qed.
-
-Lemma sep_args_sub :
-  forall Γ Ξ (xs' : list var) ts' (θ : subst_t var var) xs ts,
-    length xs = length ts ->
-    xs' = subst θ xs ->
-    ts' = subst θ ts ->
-    tc_list Γ Ξ (combine xs' ts') ->
-    var_not_in ν Γ -> 
-    wf_guards Γ Ξ ->
-    sep_env Γ && sep_guards Ξ |-- sep_env (subst θ (combine xs ts)).
-Proof.
-  intros.
-  assert (C: subst θ (combine xs ts) =
-                      combine xs' ts').
-    rewrite H0. rewrite H1.
-    rewrite <- subst_combine with (xs := xs) (ys := ts).
+    intro e'.
+    unfold subst_pred.
+    simpl. extensionality w.
+    f_equal.
+    f_equal.
+    repeat rewrite nonfree_var_expr_eval.
     reflexivity.
-    assumption.
-  rewrite C.
-  apply types_interp; assumption.
+    eauto using fresh_var_expr_fv.
+    eauto using fresh_var_expr_fv.
+  + unfold sep_pred; fold sep_pred.
+    unfold nonfreevars in *.
+    intro e.
+    rewrite subst_dist_andp.
+    rewrite subst_dist_imp.
+    f_equal.
+    rewrite <- IHp with (v := e).
+    apply  pred_ext.
+    apply derives_refl.
+    apply derives_refl.
+    inversion H1; auto.
+  + unfold sep_pred; fold sep_pred.
+    unfold nonfreevars in *.
+    intro e.
+    inversion H1.
+    repeat rewrite subst_dist_andp.
+    repeat f_equal.
+    auto.
+    auto.
+  + unfold sep_pred; fold sep_pred.
+    unfold nonfreevars in *.
+    intro e.
+    inversion H1.
+    repeat rewrite subst_dist_andp.
+    repeat rewrite subst_dist_orp.
+    repeat f_equal.
+    auto.
+    auto.
 Qed.
 
-Lemma sep_env_cons :
-  forall x t Γ,
-    sep_ty (var_e x) t * sep_env Γ |-- sep_env ((x,t) :: Γ).
+Hint Constructors wf_expr : wf.
+Hint Constructors wf_prop : wf.
+
+Lemma wf_expr_cons :
+  forall G H xt e,
+    wf_expr G H e -> wf_expr (xt :: G) H e.
 Proof.
   intros.
-  unfold sep_env at 2. fold sep_env.
-  rewrite <- sepcon_emp at 1.
-  rewrite <- sepcon_pure_andp.
-  rewrite <- sepcon_pure_andp.
-  apply sepcon_derives.
-  apply sepcon_derives.
-  apply derives_refl.
-  apply derives_refl.
-  apply derives_refl.
-  apply sep_ty_pure.
-  apply sep_env_pure.
-  unfold pure. apply andp_left1. apply sep_ty_pure.
-  apply derives_refl.
-Qed.
-  
-Lemma sep_env_cons_sub :
-  forall x b p θ Γ,
-    θ ν = ν -> (forall x , θ x = ν -> x = ν) ->
-    subst θ (sep_ty (var_e x) { ν : b | p }) * sep_env Γ
-    |-- sep_env ((subst θ (x,{ ν : b | p })) :: Γ).
-Proof.
-  intros x b p θ Γ vv_id vv_im.
-  unfold sep_env; fold sep_env.
-  rewrite sepcon_pure_andp.
-  simpl.
-  intro w.
-  apply andp_right.
-  apply andp_derives.
-  rewrite subst_lift_assert.
-  rewrite <- subst_ty_distr. 
-  unfold sep_ty. simpl.
-  apply andp_derives.
-  apply andp_derives.
-  unfold subst, Subst_var_var. apply derives_refl.
-  unfold subst. simpl.
-  rewrite subst_lift_pred. unfold subst. simpl. apply derives_refl.
-  apply derives_refl.
-  rewrite vv_id. reflexivity.
-  apply subst_vv_not_in_range.
-  intro v. split. apply vv_im. intro. rewrite H. assumption.
-  apply derives_refl.
-  apply andp_left2. apply sep_env_pure.
-  apply sep_ty_pure_subst.
-  apply sep_env_pure.
+  induction e. 
+  + constructor.
+  + inversion H0; subst; eauto with datatypes wf.
+      unfold var_in in *;
+    destruct H4; constructor; exists x; eauto with datatypes wf.
+  + inversion H0; subst; eauto with wf datatypes.
 Qed.
 
-Lemma sep_proof_proc_ret :
-  forall (θ : subst_t var var) x t Γ, 
-    θ ν = ν -> (forall x, θ x = ν -> x = ν) ->
-    wf_type (subst θ (x,t) :: Γ) (subst θ t)  ->
-   (subst θ (sep_ty (var_e x) t)) * sep_env Γ |--
-    sep_env ((subst θ (x,t)) :: Γ).
+Hint Resolve wf_expr_cons : wf.
+
+Lemma wf_prop_cons :
+  forall G H xt p,
+    wf_prop G H p -> wf_prop (xt :: G) H p.
 Proof.
-  intros θ x t Γ vvid vvim wf H.
-  destruct t as [ b p ].
+  intros.
+  induction p; inversion H0; eauto with wf.
+Qed.
+
+Hint Transparent wf_type.
+Hint Resolve wf_prop_cons : wf.
+Hint Constructors wf_env : wf.
+
+Lemma wf_type_cons :
+  forall G H xt b p ,
+    wf_type G H { ν : b | p } -> wf_type (xt :: G) H { ν : b | p }.
+Proof.
+  intros.
+  unfold wf_type in *.
   simpl in *.
-  apply sep_env_cons_sub. 
-  assumption.
-  assumption.
+  destruct b; eauto with wf.
+  destruct H0.
+  split; eauto with wf.
 Qed.
 
-Lemma sep_proof_proc_sub :
-  forall x v θ,
-    v  = subst θ x ->
-    (forall x', θ x' = v <-> x = x') ->
-    unique_sub θ x.
-Proof.
-  intros x v θ vdef subprop.
-  unfold unique_sub.
-  exists v.
-  split.
-  symmetry. apply vdef.
-  intros.
-  unfold not_free_in.
-  specialize (subprop x0).
-  destruct subprop.
-  intuition.
-  apply H.
-  symmetry.
-  intuition.
-Qed.
-
-Lemma sep_proof_proc_mod :
-  forall f xs x x',
-    modvars (proc_s f xs x []) x' -> x = x'.
+Hint Resolve wf_type_cons : wf.
+Hint Constructors reft_type.
+    
+Lemma wf_ty_mem :
+  forall G H x b p,
+    (x, { ν : b | p }) ∈ G ->
+    wf_env H G ->
+    wf_type G H { ν : b | p }.
 Proof.
   intros.
-  inversion H.
-  intuition.
-  reflexivity.
+  induction G as [ | [x' [b' p']]]; subst.
+    + contradiction.
+    + apply in_inv in H0. destruct H0. inversion H0. subst.
+      inversion H1; subst.
+      assumption.
+      inversion H1. subst. eauto with wf.
 Qed.
 
-Ltac wfenv_ty_t :=
+Hint Resolve wf_ty_mem : wf.
+
+Lemma wf_prop_from_ty :
+  forall G H b p,
+    wf_type G H { ν : b | p } -> wf_prop G H p.
+Proof.
+  intros.
+  destruct b; apply H0.
+Qed.
+
+Hint Resolve wf_prop_from_ty : wf.
+
+Ltac split_subst_var :=
   match goal with 
-    | [ X : ?x = ?a, Y : ?y = ?b, H : wf_type _ _ |- _ ] =>
-      rewrite X in H; rewrite Y in H; assumption
-    | [ H : (?x, ?y) = subst _ (_, _) |- _ ] => 
-      unfold subst, Subst_prod, subst_prod in H; inversion H; wfenv_ty_t
-    | [ H : wf_env (subst ?x (?f ?z) :: ?G) |- wf_type (subst ?x (?f ?z) :: ?G) _ ]  =>
-      inversion H; destruct (f z); simpl in *; wfenv_ty_t
+    | |- appcontext[_ (subst_one ?x _) (var_e ?v)] =>
+      unfold subst; unfold subst_one; simpl;
+      destruct (eq_dec v x); subst
   end.
 
-Lemma lift_assert :
-  forall {P Q : assert} w, P |-- Q ->(P w |-- Q w).
+Lemma subst_expr_fun :
+  forall (s : var -> expr) f e1 e2,
+    subst s (fun_e f e1 e2) = fun_e f (subst s e1) (subst s e2).
 Proof.
-  intros.
-  apply H.
+  firstorder.
 Qed.
 
-Lemma sep_proof_proccall :
-  forall Φ Ξ Γ Γ' f xs v (J : (Φ ; Γ ; Ξ) ⊢ proc_s f xs v [] ::: Γ'),
-    wf_env Γ ->
-    wf_guards Γ Ξ ->
-    sep_proc_env Φ |- {{ sep_env Γ * sep_guards Ξ }} proc_s f xs v [] {{ sep_env Γ' * sep_guards Ξ }}.
+Lemma subst_prop_rel :
+  forall (s : var -> expr) e1 e2,
+    subst s (eq_r e1 e2) = eq_r (subst s e1) (subst s e2).
+Proof. firstorder. Qed.
+
+Lemma subst_prop_not :
+  forall (s : var -> expr) p,
+    subst s (not_r p) = not_r (subst s p).
 Proof.
-  intros until v. 
-  intros J wf wfg.
-  inversion J as [ | ? ? ? ? ? p S ? ? θ θS fmem wfS wfθ 
-                     ? ? ? ? retid substid wfenv wfsubty tclist
-                     | | | ]. 
-  simpl in *. subst.
-  destruct S as [fxs fts [rx rt]] eqn:S_def.
-  simpl in *.
-  apply funspec_interp in fmem.
-  unfold sep_schema in fmem. 
-  apply semax_pre_post with 
-  (P' := ((Subst.subst θ (sep_env (combine fxs fts)))) * (sep_env Γ * sep_guards Ξ)) 
-  (Q' := ((Subst.subst θ (sep_ty (var_e rx) rt))) * (sep_env Γ * sep_guards Ξ)).
-  intro w.
-  simpl.
-  rewrite <- (subst_in_env Γ).
-  rewrite sepcon_pure_andp at 1.
-2: purity.
-2: purity.
-  rewrite (sepcon_pure_andp (sep_env (subst θ (combine fxs fts)) w)). 
-2: purity.
-2: purity.
-  apply andp_right.
-  pose sep_args_sub as argstc; simpl in argstc; apply argstc with (xs' := subst θ fxs) (ts' := subst θ fts).
-  inversion wfS; assumption.
-  reflexivity.
-  reflexivity.
-  assumption.
-  apply wf_env_no_vv; assumption.
-  assumption.
-  rewrite sepcon_pure_andp; try apply derives_refl; purity.
-  wfsubst θ.
-  assumption.
-  assumption.
-  rewrite subst_combine.
-  apply forall_p_combine.
-  inversion wfS; repeat rewrite <- subst_length; assumption.
-  assumption.
-  inversion wfS; assumption.
-  rewrite <- sepcon_assoc.
-  simpl.
-  intro w.
-  apply sepcon_derives.
-  pose sep_proof_proc_ret as RT; simpl in RT; apply RT.
-  apply wfθ; reflexivity.
-  apply wfθ.
-  inversion wfenv; assumption.
-  apply derives_refl.
-  apply semax_frame.
-  subst.
-  assert (A : subst θ (proc_s f fxs rx []) = proc_s f (subst θ fxs) (subst θ rx) []).
-  unfold subst at 1. simpl. reflexivity.
-  rewrite <- A.
-  apply semax_subst.
-  apply (semax_proc f (mkProc fxs rx [] p)).
-  assumption.
-  intros.
-  assert (rx = x) by 
-      (apply sep_proof_proc_mod with (f:=f) (xs:= fxs); assumption).
-  subst.
-  apply sep_proof_proc_sub with (v := subst θ x).
-  reflexivity.
-  intros.
-  specialize (retid x').
-  constructor; intro; [ symmetry | idtac ]; apply retid; [ idtac | symmetry]; assumption.
-  unfold subset.
-  intros.
-  unfold nonfreevars.
-  intros.
-  assert (A : subst θ rx = x).
-    apply sep_proof_proc_mod with (f := f) (xs := subst θ fxs).
-    assumption.
-  assert (B : x <> ν).
-    inversion wfenv.
-    rewrite <- A.
-    assumption.
-  rewrite sepcon_pure_andp.
-2: purity.
-2: purity.
-  rewrite subst_distr_andp.
-  apply andp_derives.
-  simpl.
-  unfold subst, Subst_pred.
-  intro w.
-  rewrite subst_dom_env.
-    apply derives_refl.
-    assumption.
-    apply subst_one_is_disj.
-    assumption.
-    assumption.
-    inversion wfenv. rewrite <- A. assumption.
-    unfold subst_one. foo.
-  intro w.
-  rewrite subst_dom_guards with (Γ := Γ).
-  apply derives_refl.
-  assumption.
-  apply subst_one_is_disj.
-  assumption.
-  assumption.
-  inversion wfenv. rewrite <- A. assumption.
+  firstorder.
 Qed.
 
-Lemma subtype_same_base :
-  forall Ξ Γ b b' p p',
-    subtype Γ Ξ { ν : b | p } { ν : b' | p' } ->
-    subtype Γ Ξ { ν : b | p } { ν : b | p' }.
+Lemma subst_prop_and :
+  forall (s : var -> expr) p1 p2,
+    subst s (and_r p1 p2) = and_r (subst s p1) (subst s p2).
 Proof.
-  intros.
-  inversion H.
-  subst.
-  assumption.
+  firstorder.
 Qed.
 
-Lemma types_interp2 :
-  forall Ξ Γ Γ', 
-    wf_env Γ -> wf_guards Γ Ξ ->
-   (forall x t, (x,t) ∈ Γ' -> (exists t1, (x,t1) ∈ Γ /\ subtype Γ Ξ t1 t)) ->
-   sep_env Γ && sep_guards Ξ |-- sep_env Γ'.
+Lemma subst_prop_or :
+  forall (s : var -> expr) p1 p2,
+    subst s (or_r p1 p2) = or_r (subst s p1) (subst s p2).
 Proof.
-  intros Ξ Γ Γ' wfe wfg H.
-  induction Γ' as [| [x t]].
-  + apply andp_right. normalize. purity.
-  + unfold sep_env; fold sep_env.
-    apply andp_right.
-    apply andp_right.
-    specialize (H x t).
-    destruct H. left. reflexivity.
-    destruct t as [b p].
-    destruct x0 as [b0 p0].
-    apply derives_trans with (Q := sep_env Γ && sep_guards Ξ && sep_ty (var_e x) {ν : b | p0}).
-    apply andp_right. trivial. apply type_interp.
-    apply wf_env_no_vv.
-    exact wfe.
-    constructor.
-    destruct H. inversion H0. subst.
-    apply H.
-    exact wfg.
-    rewrite imp_andp_adjoint.
-    pose subtype_interp as ST. simpl in ST. simpl. apply ST.
-    apply wf_env_no_vv.
-    exact wfe.
-    exact wfg.
-    destruct H.
-    inversion H0; subst.
-    assumption.
-    apply IHΓ'.
-    intros x0 t0 x0mem.
-    apply H.
-    right.
-    apply x0mem.
-    purity.
+  firstorder.
 Qed.
 
-Lemma join_swap :
-  forall Γ1 Γ2 Γ' Ξ,
-    join_env Ξ Γ1 Γ2 Γ' <-> join_env Ξ Γ2 Γ1 Γ'.
+Lemma wf_prop_not :
+  forall G H p, wf_prop G H p -> wf_prop G H (not_r p).
+Proof. firstorder. Qed.
+
+Lemma wf_prop_and :
+  forall G H p1 p2, 
+    wf_prop G H p1 -> wf_prop G H p2 -> wf_prop G H (and_r p1 p2).
+Proof. firstorder. Qed.
+
+Lemma wf_prop_or :
+  forall G H p1 p2, 
+    wf_prop G H p1 -> wf_prop G H p2 -> wf_prop G H (or_r p1 p2).
+Proof. firstorder. Qed.
+
+Hint Rewrite 
+     subst_prop_rel subst_expr_fun subst_prop_and subst_prop_or subst_prop_not 
+: wf.
+Hint Resolve 
+     subst_prop_rel subst_expr_fun subst_prop_and subst_prop_or subst_prop_not 
+     wf_prop_and wf_prop_or wf_prop_not 
+: wf.
+
+Lemma wf_subst_vv_expr :
+  forall G H e e',
+    wf_expr G H e -> wf_expr G H e' ->
+    wf_expr G H (subst (subst_one ν e') e).
 Proof.
   intros.
-  unfold join_env.
-  constructor.
-  intros [a [b c]].
-  split.
-  assumption.
-  split.
-  intros xt.
-  specialize (b xt).
-  rewrite and_comm.
-  apply b.
-  unfold join_var in *.
-  rewrite Forall_forall in *.
-  intros [x t].
-  intro.
-  destruct c with (x,t).
-  apply H.
-  split.
-  apply H0.
-  rewrite and_comm.
-  apply H1.
-  intros [a [b c]].
-  split.
-  assumption.
-  split.
-  intros xt.
-  specialize (b xt).
-  rewrite and_comm.
-  apply b.
-  unfold join_var in *.
-  rewrite Forall_forall in *.
-  intros [x t].
-  intro.
-  destruct c with (x,t).
-  apply H.
-  split.
-  apply H0.
-  rewrite and_comm.
-  apply H1.
+  induction e.
+  + eauto with wf.
+  + inversion H0; split_subst_var; eauto with wf.
+  + inversion H0; rewrite subst_expr_fun; eauto with wf.
+Qed.
+
+Lemma wf_expr_mem :
+  forall G H x b e1 e2, 
+    wf_env H G ->
+    (x, { ν : b | e1 .= e2 }) ∈ G ->
+    wf_expr G H e1.
+Proof.
+  intros.
+  assert (wf_type G H { ν : b | e1 .= e2 }) by eauto with wf.
+  inversion H2. inversion H6. eauto.
+Qed.
+
+Lemma wf_expr_swap :
+  forall G H e1 e2,
+    wf_prop G H (e1 .= e2) -> wf_prop G H (e2 .= e1).
+Proof.
+  intros.
+  inversion H0; eauto with wf.
+  Grab Existential Variables.
+  exact int_t.
+Qed.
+
+Hint Resolve wf_subst_vv_expr wf_expr_mem wf_expr_swap : wf.
+
+Lemma wf_subst_vv_pred :
+  forall G H p e,
+    wf_env H G ->
+    wf_expr G H e ->
+    wf_prop G H p -> 
+    wf_prop G H (subst (subst_one ν e) p).
+Proof.
+  intros.
+  induction p; inversion H2; autorewrite with wf; eauto with wf.
 Qed.
   
-Lemma join_interp :
-  forall Γ1 Γ2 Γ' Ξ ,
-    wf_env Γ1 -> wf_env Γ2 -> wf_guards Γ1 Ξ ->
-    join_env Ξ Γ1 Γ2 Γ' ->
-    (sep_env Γ1 && sep_guards Ξ) |-- sep_env Γ' && sep_guards Ξ.
+Hint Resolve wf_subst_vv_pred : wf.
+
+Lemma var_nonmem_free_ctx :
+  forall G H x, fresh x G H -> wf_env H G -> nonfreevars (sep_env G) x.
 Proof.
-  intros until Ξ.
-  intros wf1 wf2 wfg J.
+  intros G H x fr wf.
+  induction G as [| (x',t')].
+  + unfold nonfreevars. normalize.
+  + destruct t' as [b p]. 
+    assert (x' <> x).
+      apply var_not_in_not_eq with (G := G) (t := { ν : b | p }). 
+      apply fr.
+    unfold nonfreevars in *. 
+    intros.
+    unfold sep_env; fold sep_env.
+    repeat rewrite subst_dist_andp.
+    f_equal.
+    f_equal.
+    unfold sep_ty. 
+    repeat rewrite subst_dist_andp.
+    repeat f_equal.
+    unfold sep_base, subst_pred, subst_one.
+    destruct b; unfold eval_to; simpl; extensionality; repeat f_equal; try extensionality;
+      try match goal with
+          | |- appcontext[eq_dec ?x ?y] => destruct (eq_dec x y); (contradiction || reflexivity)
+          end.
+    assert (x' <> v0).
+      eapply var_not_in_not_eq. 
+    inversion wf. subst.
+    inversion H7. subst.
+    rewrite <- fresh_var_nonfree_pred. reflexivity.
+    eauto.
+    apply wf_subst_vv_pred. assumption. 
+    constructor. exists ({ ν : b | p }). left. reflexivity. (* Should automate this *)
+    assumption.
+    apply IHG; inversion wf; eauto with var wf.
+Qed.
+
+Lemma wf_heap_loc_fresh :
+  forall G H n x t, 
+    wf_heap G ((L n, (x, t)) :: H) ((L n, (x, t)) :: H) ->
+    fresh (V n) G H.
+Proof.
+  intros.
+  inversion H0. subst.
+  unfold fresh_loc in *.
+  apply H8.
+Qed.
+
+Hint Resolve wf_heap_loc_fresh : var wf.
+
+Lemma wf_heap_loc_not_in :
+  forall G H n x t, 
+    wf_heap G ((L n, (x, t)) :: H) ((L n, (x, t)) :: H) ->
+    var_not_in (V n) G.
+Proof.
+  eauto with var wf.
+Qed.
+Hint Resolve wf_heap_loc_not_in : var wf.
+
+Lemma var_nonmem_free_heap :
+  forall G H x, fresh x G H -> wf_heap G H H -> nonfreevars (sep_heap H) x.
+Proof.
+  intros.
+  induction H as [| [l [x' [b p]]]].
+  + unfold nonfreevars. normalize.
+  + assert (x' <> x).
+      eapply bind_not_in_not_eq. apply H0.
+    unfold nonfreevars in *.
+    intros.
+    unfold sep_heap; fold sep_heap.
+    destruct l eqn: Loc.
+    rewrite subst_dist_sepcon.
+    rewrite subst_dist_orp.
+    f_equal.
+    f_equal.
+    unfold eval_to. simpl. 
+    extensionality.
+    unfold subst_pred.
+    f_equal.
+    assert (fresh (V n) G H) by eauto with var.
+    assert (bind_not_in x ((L n, (x', { ν : b | p})) :: H)) by eauto with var wf.
+    unfold subst_one; simpl; destruct (eq_dec (V n) x).
+    exfalso. apply 
+    (* inversion H1. *)
+    (* unfold fresh_loc in *. *)
+    (* unfold fresh in H0. *)
+    (* unfold bind_not_in in H0. *)
+    (* simpl. unfold subst_one. simpl. *)
+    destruct (eq_dec (V n) x).
+Admitted.
+Lemma var_nonmem_free_grd :
+  forall G H g x, 
+    fresh x G H -> wf_env H G -> wf_guards G H g -> 
+    nonfreevars (sep_guards g) x.
+Proof.
+  intros.
+  induction g as [| g'].
+  + unfold nonfreevars. normalize.
+  + unfold sep_guards; fold sep_guards.
+    unfold nonfreevars. 
+    intros.
+    repeat rewrite subst_dist_andp.
+    repeat f_equal.
+    rewrite <- fresh_var_nonfree_pred.
+      reflexivity. eauto. inversion H2. unfold wf_guard in H5.
+      apply H5.
+      apply IHg. inversion H2. auto.
+Qed.
+
+Lemma var_val :
+  forall Γ x b φ, 
+    (x,{ ν : b | φ}) ∈ Γ ->
+    sep_env Γ |-- (EX v : (base_of_type b),
+                          (fun s => !!(eval s (var_e x) = val_of_base b v))).
+Proof.
+  induction Γ. 
+  intuition.
+  intuition.
+  destruct H.
+  + apply andp_left1. 
+    apply andp_left1.
+    apply andp_left1.
+    destruct b.
+    inversion H. subst. 
+    apply andp_left1.
+    apply exp_left.
+    intro bb.
+    apply andp_left1.
+    apply (exp_right bb).
+    apply derives_refl.
+  + apply andp_left1.
+    apply andp_left2.
+    fold sep_env.
+    apply IHΓ with (φ := φ).
+    assumption.
+Qed.
+
+Lemma var_eval :
+  forall Γ x b φ, 
+    (x, { ν : b | φ }) ∈ Γ -> 
+    sep_env Γ |-- (EX v : value, (fun s => !!(eval s (var_e x) = v))).
+Proof.
+  intros.
+  pose (var_val Γ x b φ H).
+  apply derives_trans with (Q := EX x0 : base_of_type b, (fun s => !!(eval s (var_e x) = val_of_base b x0))).
+  assumption.
+  apply exp_left.
+  intro xv.
+  simpl.
+  intro w.
+  apply prop_left.
+  intro.
+  rewrite H0.
+  simpl in xv.
+  apply (exp_right (val_of_base b xv)).
+  apply prop_right.
+  reflexivity.
+Qed.
+
+Lemma expr_eval :
+  forall Γ Σ Ξ e b φ,
+    expr_type Γ Σ Ξ e { ν : b | φ } ->
+    sep_env Γ |-- (EX v : value, (fun s => !!(eval s e = v))).
+Proof.
+  intros.
+  induction H.
+  * apply (exp_right v). simpl. intro. apply prop_right. reflexivity.
+  * apply var_eval with (Γ := Γ) (b := τ) (φ := φ0); assumption.
+  * apply IHexpr_type. 
+Qed.
+
+Lemma expr_eval_ty' :
+  forall Γ Σ Ξ e T,
+    expr_type Γ Σ Ξ e T ->
+    sep_env Γ |-- sep_base e (reft_base T).
+Proof.
+  intros.
+  unfold sep_base.
+  rewrite <- exp_andp1.
   apply andp_right.
-  destruct J as [wfJ [J1 J2]].
-  rewrite Forall_forall in J2.
-  unfold join_var in J2.
-  apply types_interp2.
-  assumption.
-  assumption.
-  intros x t xtmem.
-  specialize (J2 (x,t) xtmem).
-  apply J2.
-  apply andp_left2; apply derives_refl.
+  2: apply sep_env_pure.
+  dependent induction H;
+    match goal with
+      | v : value |- appcontext[EX _ : _, _] => 
+        destruct v;
+          match goal with
+            | z : _ |- _ => apply (exp_right z)
+            | _ => apply (exp_right tt)
+          end;
+          simpl; intro; normalize
+      | v : var |- _ => eapply var_val; eauto
+      | H : subtype _ _ _ _ |- _ =>
+        inversion H; subst; assumption
+    end.
 Qed.
 
-Lemma sep_proof_if_derives :
-  forall Ξ Γ Γ1 Γ2 Γ' e t g,
-    wf_env Γ ->
-    wf_env Γ1 ->
-    wf_env Γ2 ->
-    wf_guards Γ Ξ ->
-    wf_guards Γ1 Ξ ->
-    wf_guards Γ2 Ξ ->
-    join_env Ξ Γ1 Γ2 Γ' ->
-    expr_type Γ Ξ e t ->
-    (* (Φ; Γ; not_r (e .= int_v 0) :: Ξ)⊢s1 ::: (Γ1) -> *)
-    (* (Φ; Γ; (e .= int_v 0) :: Ξ)⊢s2 ::: (Γ2) -> *)
-    sep_env Γ1 * sep_guards (g :: Ξ) |-- sep_env Γ' && sep_guards Ξ.
+Lemma expr_eval_ty :
+  forall Γ Σ Ξ e b φ,
+    expr_type Γ Σ Ξ e { ν : b | φ } ->
+    sep_env Γ |-- 
+      (EX v : base_of_type b , (fun s => !!(eval s e = val_of_base b v))).
 Proof.
-  intros until g. intros wf wf1 wf2 wfg wfg1 wfg2 joinenv et.
-  unfold sep_guards; fold sep_guards.
-  rewrite sepcon_pure_andp.
-2: purity.
-2: purity.
-  repeat rewrite <- andp_assoc.
+  intros.
+  apply derives_trans with
+    (Q := sep_base e (reft_base { ν : b | φ })).
+  eapply expr_eval_ty'; eauto.
+  unfold sep_base. 
+  rewrite <- exp_andp1. apply andp_left1. normalize.
+Qed.
+
+Lemma exfalso_etype_fun :
+  forall G Σ Ξ f e1 e2 T,
+    expr_type G Σ Ξ (fun_e f e1 e2) T -> False.
+Proof.
+  intros.
+  dependent induction H.
+  auto.
+Qed.
+
+Hint Resolve 
+     expr_eval_ty
+     exfalso_etype_fun
+     expr_eval_ty'
+     expr_eval
+     var_val
+     var_eval
+: eval.
+
+Lemma subst_ty_base_pred :
+  forall v s b p,
+    subst_pred s (sep_ty (var_e v) { ν : b | p }) =
+    subst_pred s (sep_base (var_e v) b && sep_pred (subst (subst_one ν (var_e v)) p) && emp).
+Proof.
+  firstorder.
+Qed.
+
+Lemma subst_convert_expr :
+  forall v w e e',
+   ~ (FV e v) ->
+   eval w (subst (subst_one v e') e) =
+   eval (λ i : var, eval w (if eq_dec i v then e' else var_e i), hp w) e.
+Proof.
+  induction e; intros; auto.
+  unfold subst_expr. fold subst_expr.
+  rewrite subst_expr_fun. unfold subst. simpl.
+  unfold FV in H.
+  simpl in H.
+  rewrite IHe2; try rewrite IHe1; (reflexivity || eauto with datatypes).
+Qed.
+
+Lemma subst_help:
+  forall v e e' w,
+    ~ FV e v ->
+    (eval w e = eval (λ i : var, eval w (if eq_dec i v then e' else var_e i), hp w) e).
+Proof.
+  induction e.
+  + auto.
+  + intros.
+    simpl. destruct (eq_dec v0 v). subst v0. contradiction H.
+    unfold FV in *.
+    simpl in *.
+    eauto.
+    reflexivity.
+  + intros.
+    simpl.
+    unfold FV in H. simpl in H.
+    rewrite <- IHe1.
+    rewrite <- IHe2.
+    reflexivity.
+    eauto with datatypes.
+    eauto with datatypes.
+Qed.
+
+Lemma subst_expr_non_fv :
+  forall v e e',
+    ~ FV e v -> subst (subst_one v e') e = e.
+Proof.
+  induction e; intros; eauto with var.
+  + simpl. unfold subst_one. 
+    unfold subst. unfold Subst_var_expr. simpl.
+    destruct (eq_dec v0 v).
+    subst v0.
+    contradiction H. unfold FV. simpl. eauto with datatypes.
+    reflexivity.
+  + rewrite subst_expr_fun.
+    unfold FV in H.
+    simpl in H.
+    Hint Transparent FV.
+    rewrite IHe1. rewrite IHe2.
+    reflexivity.
+    eauto with datatypes.
+    eauto with datatypes.
+Qed.
+
+Lemma subst_assign_eq_true :
+  forall v b e,
+    ~ (FV e ν) ->
+    ~ (FV e v) ->
+    sep_base e b
+             |-- subst_pred (subst_one v e) (sep_ty (var_e v) {ν : b | var_e ν .= e}).
+Proof.
+  intros.
+  rewrite subst_ty_base_pred.
+  repeat rewrite subst_dist_andp.
+  repeat apply andp_right. 
+    unfold subst_one, subst_pred.
+    unfold sep_base. simpl.
+    intro w. apply exp_left. intro bt.
+    apply exp_right with (x := bt).
+    destruct (eq_dec v v). apply derives_refl. congruence.
+  rewrite subst_prop_rel.
+  rewrite subst_expr_non_fv with (e := e).
+  unfold subst, Subst_var_expr, subst_one. simpl.
+  unfold subst_pred.
+  destruct (eq_dec ν ν). 
+  simpl.
+  destruct (eq_dec v v).
+  intro w.
+  rewrite subst_help with (v := v) (e' := e).
+  normalize.
+  apply sep_base_pure.
+  assumption.
+  congruence.
+  congruence.
+  assumption.
+  apply sep_base_pure.
+Qed.
+
+Lemma expr_type_wf :
+  forall G H Grds e T,
+    expr_type G H Grds e T -> wf_expr G H e.
+Proof.
+  intros.
+  induction H0.
+  + constructor.
+  + constructor. exists {ν : τ | φ}. eauto.
+  + apply IHexpr_type.
+Qed.
+
+Ltac nfv_env := 
+  match goal with
+    | H : nonfreevars _ ?v |- appcontext[subst_one ?v _] =>
+      unfold nonfreevars in H; erewrite <- H; simpl; eauto using andp_left1, andp_left2, derives_refl
+    | |- _ |-- subst_pred (subst_one ?v _) ?P =>
+      assert (nonfreevars P v); eauto using var_nonmem_free_ctx, var_nonmem_free_grd; nfv_env
+  end.
+
+Lemma sep_proof_assign :
+  forall Φ Ξ Γ Σ τ v e,
+    wf_env Σ Γ ->
+    wf_heap Γ Σ Σ ->
+    wf_guards Γ Σ Ξ ->
+    stmt_type Φ Γ Σ Ξ (assign_s v e) ((v, {ν : τ | (var_e ν) .= e})::Γ) Σ ->
+    semax (sep_proc_env Φ) 
+          (sep_env Γ && sep_guards Ξ * sep_heap Σ) 
+          (assign_s v e) 
+          (sep_env ((v, {ν : τ | (var_e ν) .= e})::Γ) && sep_guards Ξ * sep_heap Σ).
+Proof.
+  intros.
+  match goal with
+    | H : stmt_type _ _ _ _ ?s _ _ |- semax _ _ ?s _ => inversion H; subst
+  end.
+  apply semax_frame.
+  apply semax_pre_post with
+     (P' := (EX v : value, eval_to e v)
+              && subst_pred (subst_one v e) (sep_env ((v, {ν : τ | (var_e ν) .= e}) :: Γ) && sep_guards Ξ))
+     (Q' := (sep_env ((v, {ν : τ | (var_e ν) .= e}) :: Γ) && sep_guards Ξ)).
+  unfold sep_env at 2; fold sep_env.
+  normalize.
+  rewrite <- exp_andp1.
+  apply andp_right.
   apply andp_left1.
-  rewrite andp_assoc.
-  rewrite andp_comm.
-  rewrite andp_assoc.
-  apply andp_left2.
-  rewrite andp_comm.
-  apply join_interp with (Γ2 := Γ2); assumption.
+  eapply derives_trans.
+  eapply expr_eval_ty' with (T := { ν : τ | φ}); eauto.
+  unfold sep_base.
+  simpl. normalize. intros. apply exp_right with (val_of_base τ x0). unfold eval_to. normalize.
+  repeat rewrite subst_dist_andp.
+  repeat apply andp_right.
+  apply derives_trans with (Q := sep_base e τ).
+  apply andp_left1.
+  eapply expr_eval_ty' with (T := { ν : τ | φ }); eauto.
+  apply subst_assign_eq_true.
+  eapply vv_not_fv; eauto.
+  intro; eapply fresh_var_expr_fv; eauto.
+  eapply expr_type_wf; eauto.
+  nfv_env.
+  rewrite subst_emp_id; apply andp_left1; apply sep_env_pure.
+  nfv_env.
+  normalize.
+  rewrite exp_andp1; apply semax_assign.
+  unfold subset. intros. inversion H3. subst x.
+  eapply var_nonmem_free_heap; eauto.
 Qed.
+  
 
-Lemma wf_guard_expr_type1 :
-  forall Γ Ξ e t,
-    wf_env Γ ->
-    expr_type Γ Ξ e t ->
-    wf_guard Γ (e .= int_v 1).
-Proof.
-  intros.
-  split.
-  repeat constructor.
-  apply wf_expr_ty_expr with Ξ t.
-    assumption.
-  simpl. rewrite  app_nil_r.
-  apply wf_expr_ty_expr_fv with Γ Ξ t; assumption.
-Qed.
 
-Lemma wf_guard_expr_type2 :
-  forall Γ Ξ e t,
-    wf_env Γ ->
-    expr_type Γ Ξ e t ->
-    wf_guard Γ (e .= int_v 0).
+Lemma sep_proof_stmt :
+  forall Φ Ξ Γ Γ' Σ Σ' s,
+    wf_env Σ Γ ->
+    wf_heap Γ Σ Σ ->
+    wf_guards Γ Σ Ξ ->
+    stmt_type Φ Γ Σ Ξ s Γ' Σ' ->
+    sep_proc_env Φ |- {{ sep_env Γ && sep_guards Ξ * sep_heap Σ }} s {{ sep_env Γ' && sep_guards Ξ * sep_heap Σ' }}.
 Proof.
-  intros.
-  split.
-  repeat constructor.
-  apply wf_expr_ty_expr with Ξ t.
-    assumption.
-  simpl. rewrite  app_nil_r.
-  apply wf_expr_ty_expr_fv with Γ Ξ t; assumption.
+  intros until s.
+  intros wf wf_h wf_g H. induction H.
+  + (** Skip **) admit.
+  + (** f(x) **) admit.
+  + (** pad **) admit.
+  + eapply sep_proof_assign; eauto. 
+    eapply t_assign; eauto.
+  + (** alloc **) admit.
+  + (** if-then-else **) admit.
+  + (** s1;s2 **) admit.
 Qed.
+  
+(*   intros. *)
+(*   rewrite <- sepcon_pure_andp. *)
+(*   rewrite <- sepcon_pure_andp. *)
+(*   dependent induction J. *)
+(*   + apply sep_proof_skip with (Φ := Φ) (Ξ := Ξ). constructor. *)
+(*   + apply sep_proof_proccall with (Φ := Φ) (Ξ := Ξ). *)
+(*     econstructor; eauto. *)
+(*     assumption. *)
+(*     assumption. *)
+(*   + apply sep_proof_assign with (Φ := Φ) (Ξ := Ξ).  *)
+(*     econstructor; eauto. *)
+(*     assumption. *)
+(*     assumption. *)
+(*   + repeat rewrite sepcon_pure_andp. *)
+(*     apply sep_proof_if with Γ1 Γ2 { ν : int_t | p }; assumption. *)
+(*     purity. *)
+(*     purity. *)
+(*     purity. *)
+(*     purity. *)
+(*   + apply semax_seq with (Q := sep_env Γ' * sep_guards Ξ). *)
+(*     apply IHJ1; assumption. *)
+(*     apply IHJ2.  *)
+(*     apply wf_env_stmt with (P := Φ) (G := Γ) (X := Ξ) (s := s1); assumption. *)
+(*     apply wf_guards_stmt with (P := Φ) (G := Γ) (X := Ξ) (s := s1); assumption. *)
+(*  + apply sep_env_pure. *)
+(*  + apply sep_guard_pure. *)
+(*  + apply sep_env_pure. *)
+(*  + apply sep_guard_pure. *)
+(* Qed. *)
 
-Lemma sep_proof_if :
-  forall Φ Ξ Γ Γ1 Γ2 Γ' s1 s2 e t,
-    wf_env Γ ->
-    wf_guards Γ Ξ ->
-    expr_type Γ Ξ e t ->
-    (Φ; Γ; (e .= int_v 1) :: Ξ)⊢s1 ::: (Γ1) ->
-    (Φ; Γ; (e .= int_v 0) :: Ξ)⊢s2 ::: (Γ2) ->
-    join_env Ξ Γ1 Γ2 Γ' ->
-    (wf_env Γ
-         → wf_guards Γ ((e .= int_v 1) :: Ξ)
-           → sep_proc_env Φ |- 
-             {{sep_env Γ * sep_guards ((e .= int_v 1) :: Ξ)}}s1
-             {{sep_env Γ1 * sep_guards ((e .= int_v 1) :: Ξ)}}) ->
-    (wf_env Γ
-       → wf_guards Γ ((e .= int_v 0) :: Ξ)
-         → sep_proc_env Φ |- 
-           {{sep_env Γ * sep_guards ((e .= int_v 0) :: Ξ)}}s2
-           {{sep_env Γ2 * sep_guards ((e .= int_v 0) :: Ξ)}}) ->
-    sep_proc_env Φ |- {{ sep_env Γ && sep_guards Ξ }} 
-                        if_s e s1 s2 
-                        {{ sep_env Γ' && sep_guards Ξ }}.
-Proof.
-  intros until t.
-  intros wf wfg et H1 H2 joinenv IH1 IH2.
-  assert (WF1 : wf_env Γ1).
-    apply wf_env_stmt with Φ Γ ((e .= int_v 1) :: Ξ) s1; assumption.
-  assert (WF2 : wf_env Γ2).
-    apply wf_env_stmt with Φ Γ (((e .= int_v 0)) :: Ξ) s2; assumption.
-  assert (WFG1 : wf_guards Γ1 ((e .= int_v 1) :: Ξ)).
-    apply wf_guards_stmt with Φ Γ s1. assumption. assumption.
-    apply Forall_cons. 
-      apply wf_guard_expr_type1 with Ξ t; assumption. 
-      assumption.
-  assert (WFG2 : wf_guards Γ2 ((e .= int_v 0) :: Ξ)).
-    apply wf_guards_stmt with Φ Γ s2. assumption. assumption.
-    apply Forall_cons. 
-      apply wf_guard_expr_type2 with Ξ t; assumption. 
-      assumption.
-  apply semax_if.
-  rewrite andp_comm.
-  rewrite andp_assoc.
-  rewrite andp_comm with (P := sep_guards Ξ).
-  apply semax_pre_post with (P' := sep_env Γ * sep_guards ((e .= int_v 1) :: Ξ))
-                            (Q' := sep_env Γ1 * sep_guards ((e .= int_v 1) :: Ξ)).
-  rewrite sepcon_pure_andp.
-    repeat apply andp_right.
-    apply andp_left1. apply derives_refl.
-    apply andp_left2. apply andp_left1. 
-    unfold eval_to. simpl. intro. apply andp_left1. apply derives_refl.
-    apply andp_left1. purity.
-    fold sep_guards.
-    do 2 apply andp_left2. apply derives_refl.
-    apply andp_left1. purity.
-    purity.
-    apply sep_guard_pure.
-  apply sep_proof_if_derives with Γ Γ2 e t.  
-    assumption.
-    assumption.
-    assumption.
-    assumption.
-    inversion WFG1; assumption.
-    inversion WFG2; assumption.
-    assumption.
-    assumption.
-  apply IH1.
-  assumption.
-  apply Forall_cons.
-    apply wf_guard_expr_type1 with Ξ t; assumption.
-    assumption.
-  apply semax_pre_post with (P' := sep_env Γ * sep_guards ((e .= int_v 0) :: Ξ))
-                            (Q' := sep_env Γ2 * sep_guards ((e .= int_v 0) :: Ξ)).
-    rewrite sepcon_pure_andp.
-    repeat apply andp_right.
-    apply andp_left2. apply andp_left1. apply derives_refl.
-    apply andp_left1. unfold eval_to. intro. apply andp_left1. apply derives_refl.
-    apply andp_left2. purity.
-    fold sep_guards.
-    apply andp_left2. apply andp_left2. apply derives_refl.
-    apply andp_left2. purity.
-    purity.
-    apply sep_guard_pure.
-  apply sep_proof_if_derives with Γ Γ1 e t;
-    repeat first [ assumption | inversion WFG1; assumption | inversion WFG2; assumption].
-  apply join_swap. assumption.
-  apply IH2.
-  assumption.
-  apply Forall_cons.
-    apply wf_guard_expr_type2 with Ξ t; assumption.
-    assumption.
-Qed.
-
-Theorem sep_proof_stmt :
-  forall Φ Ξ Γ Γ' s (J : (Φ ; Γ ; Ξ) ⊢ s ::: Γ'),
-    wf_env Γ ->
-    wf_guards Γ Ξ ->
-    sep_proc_env Φ |- {{ sep_env Γ && sep_guards Ξ }} s {{ sep_env Γ' && sep_guards Ξ }}.
-Proof.
-  intros.
-  rewrite <- sepcon_pure_andp.
-  rewrite <- sepcon_pure_andp.
-  dependent induction J.
-  + apply sep_proof_skip with (Φ := Φ) (Ξ := Ξ). constructor.
-  + apply sep_proof_proccall with (Φ := Φ) (Ξ := Ξ).
-    econstructor; eauto.
-    assumption.
-    assumption.
-  + apply sep_proof_assign with (Φ := Φ) (Ξ := Ξ). 
-    econstructor; eauto.
-    assumption.
-    assumption.
-  + repeat rewrite sepcon_pure_andp.
-    apply sep_proof_if with Γ1 Γ2 { ν : int_t | p }; assumption.
-    purity.
-    purity.
-    purity.
-    purity.
-  + apply semax_seq with (Q := sep_env Γ' * sep_guards Ξ).
-    apply IHJ1; assumption.
-    apply IHJ2. 
-    apply wf_env_stmt with (P := Φ) (G := Γ) (X := Ξ) (s := s1); assumption.
-    apply wf_guards_stmt with (P := Φ) (G := Γ) (X := Ξ) (s := s1); assumption.
- + apply sep_env_pure.
- + apply sep_guard_pure.
- + apply sep_env_pure.
- + apply sep_guard_pure.
-Qed.
-
-Corollary type_safety_stmt :
-  forall Φ Γ s, (Φ ; [] ; []) ⊢ s ::: Γ -> sep_proc_env Φ |- {{ emp }} s {{ TT }}.
-Proof.
-  intros.
-  assert (wf_env nil). constructor.
-  assert (wf_guards nil nil). constructor.
-  apply semax_pre_post with (P' := sep_env nil && sep_guards nil) 
-                            (Q' := sep_env Γ && sep_guards nil);
-  first [ apply sep_proof_stmt with (Φ := Φ) (Ξ := []); assumption
-        | unfold sep_guards; normalize ].
-Qed.
+(* Corollary type_safety_stmt : *)
+(*   forall Φ Γ s, (Φ ; [] ; []) ⊢ s ::: Γ -> sep_proc_env Φ |- {{ emp }} s {{ TT }}. *)
+(* Proof. *)
+(*   intros. *)
+(*   assert (wf_env nil). constructor. *)
+(*   assert (wf_guards nil nil). constructor. *)
+(*   apply semax_pre_post with (P' := sep_env nil && sep_guards nil)  *)
+(*                             (Q' := sep_env Γ && sep_guards nil); *)
+(*   first [ apply sep_proof_stmt with (Φ := Φ) (Ξ := []); assumption *)
+(*         | unfold sep_guards; normalize ]. *)
+(* Qed. *)
 
 Theorem sep_proof_program :
   forall Φ p,
     prog_type Φ p -> semax_prog (sep_proc_env Φ) p.
 Proof.
-  intros Φ p H.
-  induction H.
-  + constructor.
-    apply type_safety_stmt with Γ; assumption.
-  + assert (WFΓ : wf_env Γ).
-      inversion H.
-      pose (wf_env_stmt _ _ Γ _ body H9 H5).
-      apply w.
-    destruct pr. 
-    simpl in *.
-    subst.
-    pose (@semax_procdecl_p (sep_proc_env Φ)
-                           e
-                           body
-                           (sep_schema p (seq_s body (return_s e)) S)
-                           prog) as P.
-    unfold sep_schema in P.
-    destruct S.
-    destruct s_ret.
-    simpl in *.
-    simpl in *.
-    apply P.
-    reflexivity.
-    apply funspec_nomem.
-    assumption.
-    simpl in *.
-    apply semax_pre_post with (P' := sep_env (combine s_formals s_formal_ts) && sep_guards [])
-                              (Q' := sep_env Γ && sep_guards []).
-    apply andp_right. 
-      apply derives_refl. 
-      unfold sep_guards. apply andp_right. normalize. purity.
-    destruct r as [ τ φ ].
-    apply derives_trans with (Q := sep_ty (subst (subst_one v e) (var_e v)) 
-                                         (subst (subst_one v e) {ν : τ | φ})).
-    unfold subst, Subst_var_expr, subst_one at 1, Language.subst_expr.
-    destruct (eq_dec v v).
-    apply type_interp.
-    inversion H.
-    apply wf_env_no_vv. 
-    apply WFΓ.
-    assumption.
-    constructor.
-    intuition.
-    intro.
-    rewrite subst_ty_distr. apply derives_refl.
-    inversion H.
-    clear P. clear H1.
-    inversion H3.
-    unfold subst_one.
-    destruct (eq_dec ν v). intuition. subst. reflexivity.
-    assert (NEQ : v <> ν).
-    inversion H.
-    inversion H3. assumption.
-    apply subst_vv_not_in_range_exp.
-    apply wf_expr_ty_expr_fv with (Γ := Γ) (Ξ := []) (T := subst (subst_one v e) { ν : τ | φ }).
-    apply WFΓ.
-    assumption.
-    apply sep_proof_stmt in H5.
-    apply H5.
-    inversion H.
-    apply H2.
-    constructor.
-    apply IHprog_type.
-Qed.
+  Admitted.
+(*   intros Φ p H. *)
+(*   induction H. *)
+(*   + constructor. *)
+(*     apply type_safety_stmt with Γ; assumption. *)
+(*   + assert (WFΓ : wf_env Γ). *)
+(*       inversion H. *)
+(*       pose (wf_env_stmt _ _ Γ _ body H9 H5). *)
+(*       apply w. *)
+(*     destruct pr.  *)
+(*     simpl in *. *)
+(*     subst. *)
+(*     pose (@semax_procdecl_p (sep_proc_env Φ) *)
+(*                            e *)
+(*                            body *)
+(*                            (sep_schema p (seq_s body (return_s e)) S) *)
+(*                            prog) as P. *)
+(*     unfold sep_schema in P. *)
+(*     destruct S. *)
+(*     destruct s_ret. *)
+(*     simpl in *. *)
+(*     simpl in *. *)
+(*     apply P. *)
+(*     reflexivity. *)
+(*     apply funspec_nomem. *)
+(*     assumption. *)
+(*     simpl in *. *)
+(*     apply semax_pre_post with (P' := sep_env (combine s_formals s_formal_ts) && sep_guards []) *)
+(*                               (Q' := sep_env Γ && sep_guards []). *)
+(*     apply andp_right.  *)
+(*       apply derives_refl.  *)
+(*       unfold sep_guards. apply andp_right. normalize. purity. *)
+(*     destruct r as [ τ φ ]. *)
+(*     apply derives_trans with (Q := sep_ty (subst (subst_one v e) (var_e v))  *)
+(*                                          (subst (subst_one v e) {ν : τ | φ})). *)
+(*     unfold subst, Subst_var_expr, subst_one at 1, Language.subst_expr. *)
+(*     destruct (eq_dec v v). *)
+(*     apply type_interp. *)
+(*     inversion H. *)
+(*     apply wf_env_no_vv.  *)
+(*     apply WFΓ. *)
+(*     assumption. *)
+(*     constructor. *)
+(*     intuition. *)
+(*     intro. *)
+(*     rewrite subst_ty_distr. apply derives_refl. *)
+(*     inversion H. *)
+(*     clear P. clear H1. *)
+(*     inversion H3. *)
+(*     unfold subst_one. *)
+(*     destruct (eq_dec ν v). intuition. subst. reflexivity. *)
+(*     assert (NEQ : v <> ν). *)
+(*     inversion H. *)
+(*     inversion H3. assumption. *)
+(*     apply subst_vv_not_in_range_exp. *)
+(*     apply wf_expr_ty_expr_fv with (Γ := Γ) (Ξ := []) (T := subst (subst_one v e) { ν : τ | φ }). *)
+(*     apply WFΓ. *)
+(*     assumption. *)
+(*     apply sep_proof_stmt in H5. *)
+(*     apply H5. *)
+(*     inversion H. *)
+(*     apply H2. *)
+(*     constructor. *)
+(*     apply IHprog_type. *)
+(* Qed. *)
